\documentclass[10pt]{article}

% --- Packages ---
\usepackage[utf8]{inputenc}
\usepackage{amsmath, amssymb, amsthm}
\usepackage{geometry}
\usepackage{fancyhdr}
\usepackage{graphicx}
\usepackage{tikz}
\usepackage{enumitem}
\usepackage{hyperref}
\usepackage{xcolor}

\begin{document}

\section{Question 1}
\subsection{(a) Prove $a + d = p + q$}
Assume $x = \overline{AE} = \overline{EB}$ \\
Make a point $G$ on $\overline{AB}$ which $\overline{GF} \perp \overline{AB}$ \\

\begin{gather}
    \because a + d = \frac{1}{2} * x * \overline{GF} \text{ and } p + q = \frac{1}{2} * x * \overline{GF} \\
    \therefore a + d = p + q
\end{gather}

\subsection{(b) Prove $a + r = c + p$}
Assume $y = \overline{DF} = \overline{FC}$ \\
Make a point $H$ on $\overline{DC}$ which $\overline{HE} \perp \overline{DC}$ \\

\begin{gather}
    \because c + d = \frac{1}{2} * y * \overline{HE} \text{ and } r + q = \frac{1}{2} * y * \overline{HE} \\
    \therefore c + d = q + r
\end{gather}

We can use Equation (2) - Equation (4), we get:
\begin{gather}
    a + d - c - d = p + q - q - r \\
    a - c = p - r \\
    a + r = p + c 
\end{gather}

\end{document}