\subsection{Continuity and Limits}
\begin{definition}
    [Limits Law]
    Assume we have function $f(x)$ and $g(x)$, which 
    \[
        \lim_{x \to a} f(x) \text{ and } \lim_{x \to a} g(x) \text{ both exist}
    \]
    We also have constant $c$
    We get these properties:
    \begin{enumerate}
        \item \[\lim_{x\to a} c = c\]
        \item \[\lim_{x \to a} x = a\]
        \item \[
            \lim_{x \to a} \left[f(x) + g(x) \right] = \lim_{x \to a} f(x) + \lim_{x \to a} g(x)
        \]
        \item \[
            \lim_{x \to a} \left[f(x) - g(x) \right] = \lim_{x \to a} f(x) - \lim_{x \to a} g(x)
        \]
        \item \[
            \lim_{x \to a} \left[f(x) * g(x) \right] = \lim_{x \to a} f(x) * \lim_{x \to a} g(x)
        \]
        \item \[
            \lim_{x \to a}\frac{f(x)}{g(x)} = \frac{
                \lim_{x \to a} f(x) 
            }{
                \lim_{x \to a} g(x)
            }  
        \]
        \item \[
        \lim_{x \to a} \left[f(x)\right]^n = (\lim_{x \to a}f(x))^n 
        \]
        \item \[
        \lim_{x \to a} \sqrt[n]{f(x)} = \sqrt[n]{(\lim_{x \to a}f(x))} 
        \]
    \end{enumerate}
\end{definition}

Somes cases you should be careful
\begin{example}
    Evaluate and simplify
    \[
        \lim_{x \to a} \sqrt{x}
    \]
    Recall: if a limit exist
    \begin{enumerate}
        \item \[ \lim_{x \to a^{-}} f(x) \text{ exists}\]
        \item \[ \lim_{x \to a^{+}} f(x) \text{ exists}\]
        \item \[ \lim_{x \to a^{-}} f(x) = \lim_{x \to a^{+}} f(x)\]
    \end{enumerate}
    In this case, \[ \lim_{x \to 0^{-}} \sqrt{x} \text{ does not exist}\] because 
    \[
        D: {x \in \mathcal{R} | x \geq 0}
    \]
\end{example}

\begin{example}
    Evaluate and simplify: 
    \[
        \lim_{x \to 1} x^2 - 5x
    \]
    \begin{remark}
        Please be carefull with the bracket, don't mix with 
        \[
            \lim_{x \to 1} (x^2 - 5x)
        \]
    \end{remark}
    The solution should be:
    \begin{gather*}
        = (\lim_{x \to 1}x)^2 - 5x \\
        = (1)^2 - 5x\\
        = 1 - 5x
    \end{gather*}
\end{example}